src/high/locations.v
@@ -223,13 +223,16 @@ Section mapsto_at_lemmas.
       "viewFact" ∷ (have_FV_strong ℓ (tF - offset) ∨
                     persisted_loc_d ℓ (tF - offset))%I.
 
+  (* Definition pview_lb_high ℓ t: dProp Σ := *)
+  (*   lift_d (λ nD, own pview_lb_name (◯ {[ ℓ := MaxNat t ]})). *)
+
   Program Definition persist_lb ℓ prot (sP : ST) : dProp Σ :=
     ∃ tP offset,
       "#lbBase" ∷ lb_base ℓ prot offset tP sP ∗
       (* We have the persisted state in our store view. *)
       "#tPLe" ∷ have_FV ℓ (tP - offset) ∗
-      "persisted" ∷ persisted_loc_d ℓ (tP - offset) ∗
-      "#pview_lb" ∷ lift_d (λ nD, ℓ ↪[pview_lb_name]□ tP).
+      "persisted" ∷ persisted_loc_d ℓ (tP - offset).
+      (* "#pview_lb_high" ∷ pview_lb_high ℓ (tP - offset). *)
 
   Definition crashed_in prot ℓ s : dProp Σ :=
     ∃ CV,
@@ -448,7 +451,7 @@ Section mapsto_at_lemmas.
     iFrameF (slice). iFrame "physMsg". iFrame "inThreadView".
     iSplitPure; first done.
     iFrameF (haveTStore).
-    iLeft. iApply persisted_loc_d_weak. last done. lia.
+    iLeft. iApply persisted_loc_d_weak; last done. lia.
   Qed.
 
   Lemma mapsto_na_persist_lb_last ℓ prot q ss s `{!AntiSymm (=) (⊑@{ST})} :
