src/high/resources.v
@@ -72,7 +72,7 @@ Class nvmHighFixedG Σ := {
   offsetsG :> ghost_mapG Σ loc nat;
   locsG :> inG Σ shared_locsR;
   nvm_bumpersG :> bumpersG Σ;
-  pview_lbG :> ghost_mapG Σ loc max_nat;
+  pview_lbG :> inG Σ (authR viewUR);
 }.
 
 Definition nvmHighΣ :=
@@ -85,7 +85,7 @@ Definition nvmHighΣ :=
      ghost_mapΣ loc nat;
      GFunctor (shared_locsR);
      ghost_mapΣ loc (positive → option positive);
-     ghost_mapΣ loc max_nat
+     GFunctor (authRF viewUR)
     ].
 
 Instance subG_nvmHighΣ {Σ} : subG nvmHighΣ Σ → nvmHighFixedG Σ.
@@ -113,6 +113,7 @@ Definition get_bumpers_name (gnames : nvmDeltaG) := bumpers_name.
 Definition get_at_locs_name (gnames : nvmDeltaG) := shared_locs_name.
 Definition get_na_locs_name (gnames : nvmDeltaG) := exclusive_locs_name.
 Definition get_na_views_name (gnames : nvmDeltaG) := non_atomic_views_gname.
+Definition get_pview_lb_name (gnames : nvmDeltaG) := pview_lb_name.
 
 (* Wrappers around ownership of resources that extracts the ghost names from
    [nvmDeltaG]. These wrapper makes it easier to switch the ghost names around
